Small_Step.thy
@@ -13,11 +13,30 @@ Seq2:   "(Some(c0), s) \<rightarrow> (Some(c2), t) \<Longrightarrow> (Some (c0;;
 IfTrue:  "bval b s \<Longrightarrow> (Some({P} IF b THEN c1 ELSE c2 FI), s) \<rightarrow> (Some(c1), s)" |
 IfFalse: "\<not>bval b s \<Longrightarrow> (Some({P} IF b THEN c1 ELSE c2 FI), s) \<rightarrow> (Some(c2), s)" |
 
-WhileTrue: "\<not>bval b s \<Longrightarrow> (Some ({P} WHILE b INV I DO c OD), s) \<rightarrow> (None, s)" |
-WhileFalse:"bval b s \<Longrightarrow> (Some({P} WHILE b INV I DO c OD), s) \<rightarrow> (Some(c;; ({I} WHILE b INV I DO c OD)), s)"|
+WhileFalse: "\<not>bval b s \<Longrightarrow> (Some ({P} WHILE b INV I DO c OD), s) \<rightarrow> (None, s)" |
+WhileTrue:"\<lbrakk>bval b s; \<forall>s. P s \<longrightarrow> I s; \<forall>s. I s \<and> bval b s \<longrightarrow> pre(c) s\<rbrakk> \<Longrightarrow> (Some({P} WHILE b INV I DO c OD), s) \<rightarrow> (Some(c;; ({I} WHILE b INV I DO c OD)), s)"|
 
 Wait:"bval b s \<Longrightarrow> (Some({P} WAIT b END), s) \<rightarrow> (None, s)"
 
+inductive
+  big_step :: "(acom option) * state \<Rightarrow> state \<Rightarrow> bool" (infix "\<Rightarrow>" 55)
+where
+BNone: "(None, t) \<Rightarrow> t"|
+
+Assign:  "(Some({P} x ::= a), s) \<Rightarrow> s(x := aval a s)" |
+
+Seq:   "\<lbrakk>(Some(c0), s) \<Rightarrow> t; (Some(c1), t) \<Rightarrow> r\<rbrakk> \<Longrightarrow> (Some (c0;; c1), s) \<Rightarrow> r" |
+
+IfTrue:  "\<lbrakk>bval b s; (Some(c1), s) \<Rightarrow> t\<rbrakk> \<Longrightarrow> (Some({P} IF b THEN c1 ELSE c2 FI), s) \<Rightarrow> t" |
+IfFalse: "\<lbrakk>\<not>bval b s; (Some(c2), s) \<Rightarrow> t\<rbrakk> \<Longrightarrow> (Some({P} IF b THEN c1 ELSE c2 FI), s) \<Rightarrow> t" |
+
+WhileFalse: "\<not>bval b s \<Longrightarrow> (Some ({P} WHILE b INV I DO c OD), s) \<Rightarrow> s" |
+WhileTrue:"\<lbrakk>bval b s; \<forall>s. P s \<longrightarrow> I s; \<forall>s. I s \<and> bval b s \<longrightarrow> pre(c) s; (Some c, s) \<Rightarrow> s1; (Some({I} WHILE b INV I DO c OD), s1) \<Rightarrow> t\<rbrakk> \<Longrightarrow> (Some({P} WHILE b INV I DO c OD), s) \<Rightarrow> t"|
+
+Wait:"bval b s \<Longrightarrow> (Some({P} WAIT b END), s) \<Rightarrow> s"
+
+code_pred big_step .
+lemmas big_step_induct = big_step.induct[split_format(complete)]
 
 abbreviation
   small_steps :: "(acom option) * state \<Rightarrow> (acom option) * state \<Rightarrow> bool" (infix "\<rightarrow>*" 55)
@@ -40,19 +59,24 @@ WhileTrue:"bval b s \<Longrightarrow> (Some(WHILE b INV I DO c OD), s) \<rightar
 Wait:"bval b s \<Longrightarrow> (Some(WAIT b END), s) \<rightarrow>\<^sub>t\<^sub>r (None, s)"
 
 inductive
-  big_step_tr :: "(com option) * state \<Rightarrow> (com option) * state \<Rightarrow> bool" (infix "\<Rightarrow>\<^sub>t\<^sub>r" 55)
+  big_step_tr :: "(com option) * state \<Rightarrow> state \<Rightarrow> bool" (infix "\<Rightarrow>\<^sub>t\<^sub>r" 55)
 where
-Assign:  "(Some(x ::= a), s) \<Rightarrow>\<^sub>t\<^sub>r (None, s(x := aval a s))" |
+BNone:  "(None, t) \<Rightarrow>\<^sub>t\<^sub>r t"|
 
-Seq:   "\<lbrakk>(Some(c0), s) \<Rightarrow>\<^sub>t\<^sub>r (None, t); (Some(c1), t) \<Rightarrow>\<^sub>t\<^sub>r (None, r)\<rbrakk> \<Longrightarrow> (Some (c0;; c1), s) \<Rightarrow>\<^sub>t\<^sub>r (None, r)" |
+Assign:  "(Some(x ::= a), s) \<Rightarrow>\<^sub>t\<^sub>r s(x := aval a s)" |
 
-IfTrue:  "\<lbrakk>bval b s; (Some(c1), s) \<Rightarrow>\<^sub>t\<^sub>r (None, t)\<rbrakk> \<Longrightarrow> (Some(IF b THEN c1 ELSE c2 FI), s) \<Rightarrow>\<^sub>t\<^sub>r (None, t)" |
-IfFalse: "\<lbrakk>\<not>bval b s; (Some(c2), s) \<Rightarrow>\<^sub>t\<^sub>r (None, t)\<rbrakk> \<Longrightarrow> (Some(IF b THEN c1 ELSE c2 FI), s) \<Rightarrow>\<^sub>t\<^sub>r (None, t)" |
+Seq:   "\<lbrakk>(Some(c0), s) \<Rightarrow>\<^sub>t\<^sub>r t; (Some(c1), t) \<Rightarrow>\<^sub>t\<^sub>r r\<rbrakk> \<Longrightarrow> (Some (c0;; c1), s) \<Rightarrow>\<^sub>t\<^sub>r r" |
 
-WhileFalse: "\<not>bval b s \<Longrightarrow> (Some (WHILE b INV I DO c OD), s) \<Rightarrow>\<^sub>t\<^sub>r (None, s)" |
-WhileTrue:"\<lbrakk>bval b s; (Some c, s) \<Rightarrow>\<^sub>t\<^sub>r (None, s1); (Some(WHILE b INV I DO c OD), s1) \<Rightarrow>\<^sub>t\<^sub>r (None, t)\<rbrakk> \<Longrightarrow> (Some(WHILE b INV I DO c OD), s) \<Rightarrow>\<^sub>t\<^sub>r (None, t)"|
+IfTrue:  "\<lbrakk>bval b s; (Some(c1), s) \<Rightarrow>\<^sub>t\<^sub>r t\<rbrakk> \<Longrightarrow> (Some(IF b THEN c1 ELSE c2 FI), s) \<Rightarrow>\<^sub>t\<^sub>r t" |
+IfFalse: "\<lbrakk>\<not>bval b s; (Some(c2), s) \<Rightarrow>\<^sub>t\<^sub>r t\<rbrakk> \<Longrightarrow> (Some(IF b THEN c1 ELSE c2 FI), s) \<Rightarrow>\<^sub>t\<^sub>r t" |
 
-Wait:"bval b s \<Longrightarrow> (Some(WAIT b END), s) \<Rightarrow>\<^sub>t\<^sub>r (None, s)"
+WhileFalse: "\<not>bval b s \<Longrightarrow> (Some (WHILE b INV I DO c OD), s) \<Rightarrow>\<^sub>t\<^sub>r s" |
+WhileTrue:"\<lbrakk>bval b s; (Some c, s) \<Rightarrow>\<^sub>t\<^sub>r s1; (Some(WHILE b INV I DO c OD), s1) \<Rightarrow>\<^sub>t\<^sub>r t\<rbrakk> \<Longrightarrow> (Some(WHILE b INV I DO c OD), s) \<Rightarrow>\<^sub>t\<^sub>r t"|
+
+Wait:"bval b s \<Longrightarrow> (Some(WAIT b END), s) \<Rightarrow>\<^sub>t\<^sub>r s"
+
+code_pred big_step_tr.
+lemmas big_step_tr_induct = big_step_tr.induct[split_format(complete)]
 
 abbreviation
   small_steps_tr :: "(com option) * state \<Rightarrow> (com option) * state \<Rightarrow> bool" (infix "\<rightarrow>\<^sub>t\<^sub>r*" 55)
@@ -84,6 +108,53 @@ inductive_cases small_step_cases:
     "(Some ({P} WHILE b INV I DO c OD), s) \<rightarrow> (c', s')"
     "(Some ({P} WAIT b END), s) \<rightarrow> (c', s')"
 
+
+inductive_cases BNoneE[elim!]: "(None, s) \<Rightarrow> t"
+inductive_cases BAssignE[elim!]: "(Some {P} x ::= a, s) \<Rightarrow> t"
+inductive_cases BSeqE[elim!]: "(Some c1;;c2, s1) \<Rightarrow> t"
+inductive_cases BIfE[elim!]: "(Some {P} IF b THEN c1 ELSE c2 FI, s) \<Rightarrow> t"
+inductive_cases BWhileE[elim]: "(Some {P} WHILE b INV I DO c OD, s) \<Rightarrow> t"
+inductive_cases BWaitE[elim]: "(Some {P} WAIT b END, s) \<Rightarrow> t"
+
+inductive_cases BTNoneE[elim!]: "(None, s) \<Rightarrow>\<^sub>t\<^sub>r t"
+inductive_cases BTAssignE[elim!]: "(Some x ::= a, s) \<Rightarrow>\<^sub>t\<^sub>r t"
+inductive_cases BTSeqE[elim!]: "(Some c1;;c2, s1) \<Rightarrow>\<^sub>t\<^sub>r t"
+inductive_cases BTIfE[elim!]: "(Some IF b THEN c1 ELSE c2 FI, s) \<Rightarrow>\<^sub>t\<^sub>r t"
+inductive_cases BTWhileE[elim]: "(Some WHILE b INV I DO c OD, s) \<Rightarrow>\<^sub>t\<^sub>r t"
+inductive_cases BTWaitE[elim]: "(Some WAIT b END, s) \<Rightarrow>\<^sub>t\<^sub>r t"
+
+lemma assign_simp:
+  "(Some {P} x ::= a, s) \<Rightarrow> s' <-> (s' = s(x := aval a s))"
+using big_step.Assign by auto
+ 
+
+text {* An example combining rule inversion and derivations *}
+lemma Seq_assoc:
+  "(Some (c1;; c2);; c3, s) \<Rightarrow> s' <-> (Some c1;; (c2;; c3), s) \<Rightarrow> s'"
+proof
+  assume "(Some (c1;; c2);; c3, s) \<Rightarrow> s'"
+  then obtain s1 s2 where
+    c1: "(Some c1, s) \<Rightarrow> s1" and
+    c2: "(Some c2, s1) \<Rightarrow> s2" and
+    c3: "(Some c3, s2) \<Rightarrow> s'" by auto
+  from c2 c3
+  have "(Some c2;; c3, s1) \<Rightarrow> s'" using big_step.Seq by auto 
+  with c1
+  show "(Some c1;; (c2;; c3), s) \<Rightarrow> s'" by (rule big_step.Seq)
+next
+  assume "(Some c1;; (c2;; c3), s) \<Rightarrow> s'"
+  then obtain s1 s2 where
+    c1: "(Some c1, s) \<Rightarrow> s1" and
+    c2: "(Some c2, s1) \<Rightarrow> s2" and
+    c3: "(Some c3, s2) \<Rightarrow> s'" by auto
+  from c1 c2
+  have "(Some c1;; c2, s) \<Rightarrow> s2" using big_step.Seq by auto   
+  with c3
+  show "(Some (c1;; c2);; c3, s) \<Rightarrow> s'" using big_step.Seq by auto 
+qed
+
+theorem big_step_determ: "\<lbrakk>(c,s) \<Rightarrow> t; (c,s) \<Rightarrow> u \<rbrakk> \<Longrightarrow> u = t"
+  by (induction arbitrary: u rule: big_step.induct) blast+
 
 text{* A simple property: *}
 lemma deterministic:
@@ -164,27 +235,340 @@ lemma star_seq_none:
   assumes "(Some c1, s) \<rightarrow>* (None, t)"
   shows "(Some(c1;; c2), s) \<rightarrow>* (Some c2, t)"
 using assms
-proof(induct "(Some c1)" s "None::acom option" t rule: star_induct[where r = small_step])
+proof(induct "(Some c1)" s "None::acom option" t arbitrary:c1 rule: star_induct[where r = small_step])
   case (step s y s' t)
   assume 1:"(Some c1, s) \<rightarrow> (y, s')" and 2:"(y, s') \<rightarrow>* (None, t)"
-  have "(Some(c1;; c2), s) \<rightarrow>* (Some c2, t)"
-  proof-
   {
     assume 3:"y = None"
     have "t = s'" using 2 3 none_final(2) by auto
-  (*using 1
-  proof (induct "(Some c1, s)" "(y, s')" rule:small_step.induct)
-    case (Assign P x a)
-    thus ?case using 2 none_final(2) by blast 
-  next
-    case (Seq1 c0 c1')
-    thus ?case*)
-
+    hence "(Some(c1;; c2), s) \<rightarrow>* (Some c2, t)" using 1 3 by blast
+  }
+  moreover
+  {
+    assume "y = Some c" 
+    hence "(Some(c1;; c2), s) \<rightarrow>* (Some c2, t)" by (metis 1 small_step.Seq2 star.simps step.hyps(3))
+  }
+  moreover have "(Some(c1;; c2), s) \<rightarrow>* (Some c2, t)" by (metis (full_types) 1 calculation(1) deterministic prod.inject small_step.Seq2 small_step_Pii_PoiE small_step_Pii_PoiI split_option_ex star.step step.hyps(3)) 
+  thus ?case by blast 
 qed
 
 lemma seq_comp:
   "\<lbrakk>(Some c1, s1) \<rightarrow>* (None, s2); (Some c2, s2) \<rightarrow>* (None, s3)\<rbrakk>
    \<Longrightarrow> (Some (c1;;c2), s1) \<rightarrow>* (None, s3)"
-by(blast intro: star.step star_seq2 star_trans)
+by (meson star_seq_none star_trans)
+
+lemma big_to_small:
+  "cs \<Rightarrow> t \<Longrightarrow> cs \<rightarrow>* (None, t)"
+proof (induction rule: big_step.induct)
+  case (BNone t) thus ?case by simp
+next
+  case (Assign P x a s) thus ?case by blast 
+next
+  case (Seq c1 s r c2 t)
+  assume "(Some c1, s) \<rightarrow>* (None, r)" and "(Some c2, r) \<rightarrow>* (None, t)"
+  thus ?case by (rule seq_comp)
+next
+  case (IfTrue b s c1 t P c2)
+  assume "bval b s"
+  hence "(Some {P} IF b THEN c1 ELSE c2 FI, s) \<rightarrow> (Some c1, s)"  by simp
+  moreover assume "(Some c1, s) \<rightarrow>* (None, t)"
+  ultimately 
+  show ?case by (metis star.simps)
+next
+  case (IfFalse b s c2 t P c1)
+  assume "\<not>bval b s"
+  hence "(Some {P} IF b THEN c1 ELSE c2 FI, s) \<rightarrow> (Some c2, s)" by simp
+  moreover assume "(Some c2, s) \<rightarrow>* (None, t)"
+  ultimately 
+  show ?case by (metis star.simps)
+next
+  case (WhileFalse b s P I c)
+  assume b: "\<not> bval b s"
+  show ?case by (simp add: b) 
+next
+  case (WhileTrue b s P I c s1 t)
+  let ?w  = "{I} WHILE b INV I DO c OD"
+  let ?if = "c;; {I} WHILE b INV I DO c OD"
+  assume w: "(Some ?w, s1) \<rightarrow>* (None, t)"
+  assume c: "(Some c, s) \<rightarrow>* (None, s1)"
+  assume b: "bval b s"
+  have "(Some ?w, s) \<rightarrow> (Some ?if, s)" using WhileTrue.hyps(3) b by blast 
+  moreover have "(Some ?if, s) \<rightarrow>* (None, t)" using c seq_comp w by blast 
+  ultimately show ?case by (metis WhileTrue.hyps(2) WhileTrue.hyps(3) b small_step.WhileTrue star.step) 
+next
+  case (Wait b s P)
+  thus ?case by blast 
+qed
+
+lemma  "cs \<Rightarrow> t \<Longrightarrow> cs \<rightarrow>* (None, t)"
+proof (induction rule: big_step.induct)
+  case BNone show ?case by simp
+next
+  case Assign show ?case by blast
+next
+  case Seq thus ?case by (blast intro: seq_comp)
+next
+  case IfTrue thus ?case by (blast intro: star.step)
+next
+  case IfFalse thus ?case by (blast intro: star.step)
+next
+  case WhileFalse thus ?case by simp
+next
+  case WhileTrue
+  thus ?case using big_step.WhileTrue big_to_small by blast
+next
+  case Wait thus ?case by simp
+qed
+
+lemma small_big_continue:
+  "cs \<rightarrow> cs' \<Longrightarrow> cs' \<Rightarrow> t \<Longrightarrow> cs \<Rightarrow> t"
+proof (induction arbitrary: t rule: small_step.induct)
+  case (Assign P x a s t)
+  thus ?case using big_step.Assign big_to_small final_det by blast
+next
+  case (Seq1 c1 s r c2 t)
+  thus ?case using big_step.BNone big_step.Seq by blast 
+next 
+  case (Seq2 c0 s c2 r c1 t)
+  thus ?case using big_step.Seq by blast
+next
+  case (IfTrue b s P c1 c2 t)
+  thus ?case by (simp add: big_step.IfTrue)
+next
+  case (IfFalse b s P c1 c2 t)
+  thus ?case by (simp add: big_step.IfFalse)
+next
+  case (WhileFalse b s P I c t)
+  thus ?case using big_step.WhileFalse big_to_small final_det by blast 
+next
+  case (WhileTrue b s P I c t)
+  thus ?case using big_step.WhileTrue by blast 
+next
+  case (Wait b s P t)
+  thus ?case using big_step.Wait big_to_small final_det by blast
+qed
+
+
+lemma small_to_big: "cs \<rightarrow>* (None, t) \<Longrightarrow> cs \<Rightarrow> t"
+apply (induction cs "(None::acom option, t)" rule: star.induct)
+apply (auto intro: small_big_continue)
+apply (simp add: big_step.BNone)
+done
+
+theorem big_iff_small:
+  "cs \<Rightarrow> t = cs \<rightarrow>* (None, t)"
+by(metis big_to_small small_to_big)
+
+lemma none_final_tr:
+  assumes "(None, s) \<rightarrow>\<^sub>t\<^sub>r* (c, t)"
+  shows "c = None" and "s = t"
+proof -
+  from assms have "c = None \<and> s = t"
+  proof (induction "(None::(com option), s)" "(c, t)" rule:star.induct)
+    case (step y)
+    from step.hyps(1) have "False"
+    by (induct "(None::(com option),s)" y rule:small_step_tr.induct)
+    thus ?case by auto
+  next
+    case refl
+    thus ?case by simp
+  qed
+  thus "c = None" and "s = t" by auto
+qed
+
+lemma final_det_tr:
+  assumes "(c,s) \<rightarrow>\<^sub>t\<^sub>r* (None,t)"
+  and "(c,s) \<rightarrow>\<^sub>t\<^sub>r* (None, t')"
+  shows "t = t'"
+using assms
+proof (induct "(c,s)" "(None::(com option), t)" arbitrary:c s rule:star.induct) 
+  case refl thus ?case using none_final_tr(2) by blast 
+next
+  case step thus ?case using tr_deterministic by (metis (no_types, lifting) case_prodE none_final_tr(2) split_curry star.simps)
+qed
+
+lemma star_seq2_tr:
+  assumes "(Some c1, s) \<rightarrow>\<^sub>t\<^sub>r* (Some c1', s')"
+  shows "(Some(c1;; c2), s) \<rightarrow>\<^sub>t\<^sub>r* (Some(c1';; c2), s')"
+using assms
+proof(induction "(Some c1)" s "(Some c1')" "s'" arbitrary:c1 rule: star_induct[where r = small_step_tr])
+  case refl thus ?case by simp
+next
+  case (step s con s' t)
+  from none_final_tr step.hyps(1,2) obtain c where 1:"con = Some c" by fastforce
+  with step.hyps(3) have 2:"(Some c;; c2, s') \<rightarrow>\<^sub>t\<^sub>r* (Some c1';; c2, t)" by blast
+  from 1 2 step.hyps(1) show ?case by (meson small_step_tr.Seq2 star.simps)
+qed
+
+lemma star_seq_none_tr: 
+  assumes "(Some c1, s) \<rightarrow>\<^sub>t\<^sub>r* (None, t)"
+  shows "(Some(c1;; c2), s) \<rightarrow>\<^sub>t\<^sub>r* (Some c2, t)"
+using assms
+proof(induct "(Some c1)" s "None::com option" t arbitrary:c1 rule: star_induct[where r = small_step_tr])
+  case (step s y s' t)
+  assume 1:"(Some c1, s) \<rightarrow>\<^sub>t\<^sub>r (y, s')" and 2:"(y, s') \<rightarrow>\<^sub>t\<^sub>r* (None, t)"
+  {
+    assume 3:"y = None"
+    have "t = s'" using 2 3 none_final_tr(2) by auto
+    hence "(Some(c1;; c2), s) \<rightarrow>\<^sub>t\<^sub>r* (Some c2, t)" using 1 3 by blast
+  }
+  moreover
+  {
+    assume "y = Some c" 
+    hence "(Some(c1;; c2), s) \<rightarrow>\<^sub>t\<^sub>r* (Some c2, t)" by (metis 1 small_step_tr.Seq2 star.simps step.hyps(3))
+  }
+  moreover have "(Some(c1;; c2), s) \<rightarrow>\<^sub>t\<^sub>r* (Some c2, t)" by (metis "1" calculation(1) option.exhaust small_step_tr.Seq2 star.step step.hyps(3))  
+  thus ?case by blast 
+qed
+
+lemma seq_comp_tr:
+  "\<lbrakk>(Some c1, s1) \<rightarrow>\<^sub>t\<^sub>r* (None, s2); (Some c2, s2) \<rightarrow>\<^sub>t\<^sub>r* (None, s3)\<rbrakk>
+   \<Longrightarrow> (Some (c1;;c2), s1) \<rightarrow>\<^sub>t\<^sub>r* (None, s3)"
+by (meson star_seq_none_tr star_trans)
+
+lemma big_to_small_tr:
+  "cs \<Rightarrow>\<^sub>t\<^sub>r t \<Longrightarrow> cs \<rightarrow>\<^sub>t\<^sub>r* (None, t)"
+proof (induction rule: big_step_tr.induct)
+  case (BNone t) thus ?case by simp
+next
+  case (Assign x a s) thus ?case by blast 
+next
+  case (Seq c1 s r c2 t)
+  assume "(Some c1, s) \<rightarrow>\<^sub>t\<^sub>r* (None, r)" and "(Some c2, r) \<rightarrow>\<^sub>t\<^sub>r* (None, t)"
+  thus ?case by (rule seq_comp_tr)
+next
+  case (IfTrue b s c1 t c2)
+  assume "bval b s"
+  hence "(Some IF b THEN c1 ELSE c2 FI, s) \<rightarrow>\<^sub>t\<^sub>r (Some c1, s)"  by simp
+  moreover assume "(Some c1, s) \<rightarrow>\<^sub>t\<^sub>r* (None, t)"
+  ultimately show ?case by (metis star.simps)
+next
+  case (IfFalse b s c2 t c1)
+  assume "\<not>bval b s"
+  hence "(Some IF b THEN c1 ELSE c2 FI, s) \<rightarrow>\<^sub>t\<^sub>r (Some c2, s)" by simp
+  moreover assume "(Some c2, s) \<rightarrow>\<^sub>t\<^sub>r* (None, t)"
+  ultimately show ?case by (metis star.simps)
+next
+  case (WhileFalse b s I c)
+  assume b: "\<not> bval b s"
+  show ?case by (simp add: b) 
+next
+  case (WhileTrue b s c s1 I t)
+  let ?w  = "WHILE b INV I DO c OD"
+  let ?if = "c;; WHILE b INV I DO c OD"
+  assume w: "(Some ?w, s1) \<rightarrow>\<^sub>t\<^sub>r* (None, t)"
+  assume c: "(Some c, s) \<rightarrow>\<^sub>t\<^sub>r* (None, s1)"
+  assume b: "bval b s"
+  have "(Some ?w, s) \<rightarrow>\<^sub>t\<^sub>r (Some ?if, s)" using WhileTrue.hyps(3) b by blast 
+  moreover have "(Some ?if, s) \<rightarrow>\<^sub>t\<^sub>r* (None, t)" using c seq_comp_tr w by blast 
+  ultimately show ?case by (metis WhileTrue.hyps(2) WhileTrue.hyps(3) b small_step_tr.WhileTrue star.step) 
+next
+  case (Wait b s) thus ?case by blast 
+qed
+
+lemma  "cs \<Rightarrow>\<^sub>t\<^sub>r t \<Longrightarrow> cs \<rightarrow>\<^sub>t\<^sub>r* (None, t)"
+proof (induction rule: big_step_tr.induct)
+  case BNone show ?case by simp
+next
+  case Assign show ?case by blast
+next
+  case Seq thus ?case by (blast intro: seq_comp_tr)
+next
+  case IfTrue thus ?case by (blast intro: star.step)
+next
+  case IfFalse thus ?case by (blast intro: star.step)
+next
+  case WhileFalse thus ?case by simp
+next
+  case WhileTrue
+  thus ?case using big_step_tr.WhileTrue big_to_small_tr by blast
+next
+  case Wait thus ?case by simp
+qed
+
+lemma small_big_continue_tr:
+  "cs \<rightarrow>\<^sub>t\<^sub>r cs' \<Longrightarrow> cs' \<Rightarrow>\<^sub>t\<^sub>r t \<Longrightarrow> cs \<Rightarrow>\<^sub>t\<^sub>r t"
+proof (induction arbitrary: t rule: small_step_tr.induct)
+  case (Assign x a s t)
+  thus ?case using big_step_tr.Assign big_to_small_tr final_det_tr by blast
+next
+  case (Seq1 c1 s r c2 t)
+  thus ?case using BNone big_step_tr.Seq by blast
+next 
+  case (Seq2 c0 s c2 r c1 t)
+  thus ?case using big_step_tr.Seq by blast
+next
+  case (IfTrue b s c1 c2 t)
+  thus ?case by (simp add: big_step_tr.IfTrue)
+next
+  case (IfFalse b s c1 c2 t)
+  thus ?case by (simp add: big_step_tr.IfFalse)
+next
+  case (WhileFalse b s I c t)
+  thus ?case using big_step_tr.WhileFalse big_to_small_tr final_det_tr by blast 
+next
+  case (WhileTrue b s I c t)
+  thus ?case using big_step_tr.WhileTrue by blast 
+next
+  case (Wait b s t)
+  thus ?case using big_step_tr.Wait big_to_small_tr final_det_tr by blast
+qed
+
+
+lemma small_to_big_tr: "cs \<rightarrow>\<^sub>t\<^sub>r* (None, t) \<Longrightarrow> cs \<Rightarrow>\<^sub>t\<^sub>r t"
+apply (induction cs "(None::com option, t)" rule: star.induct)
+apply (auto intro: small_big_continue_tr)
+apply (simp add: BNone)
+done
+
+theorem big_iff_small_tr:
+  "cs \<Rightarrow>\<^sub>t\<^sub>r t = cs \<rightarrow>\<^sub>t\<^sub>r* (None, t)"
+by(metis big_to_small_tr small_to_big_tr)
+
+lemma big_equal_tr:"(Some C, s) \<Rightarrow> t \<Longrightarrow> (Some (strip C), s) \<Rightarrow>\<^sub>t\<^sub>r t"
+proof(induct "(Some C, s)" t arbitrary:C s rule:big_step.induct)
+  case (Assign P x a s) 
+    thus ?case using big_step_tr.Assign by auto
+next
+  case (Seq c0 s t c1 r) thus ?case using big_step_tr.Seq by auto
+next
+  case (IfTrue b s c1 t P c2)
+    thus ?case by (simp add: big_step_tr.IfTrue)
+next
+  case (IfFalse b s c2 t P c1)
+    thus ?case by (simp add: big_step_tr.IfFalse)
+next
+  case (WhileFalse b s P I c)
+    thus ?case by (simp add: big_step_tr.WhileFalse)
+next
+  case (WhileTrue b s P I c s1 t)
+    thus ?case using big_step_tr.WhileTrue by auto
+next
+  case (Wait b s P)
+    thus ?case by (simp add: big_step_tr.Wait) 
+qed
+
+(*lemma tr_big_equal:"(Some c, s) \<Rightarrow>\<^sub>t\<^sub>r t \<Longrightarrow> \<exists>C. (strip C = c) \<and> (Some C, s) \<Rightarrow> t"
+proof(induct "(Some c, s)" t arbitrary:c s rule:big_step_tr.induct)
+  case (Assign x a s) 
+    thus ?case using big_step.Assign strip.simps(1) by blast 
+next
+  case (Seq c0 s t c1 r) thus ?case using big_step_tr.Seq by auto
+next
+  case (IfTrue b s c1 t c2)
+    thus ?case by (simp add: big_step.IfTrue)
+next
+  case (IfFalse b s c2 t P c1)
+    thus ?case by (simp add: big_step_tr.IfFalse)
+next
+  case (WhileFalse b s P I c)
+    thus ?case by (simp add: big_step_tr.WhileFalse)
+next
+  case (WhileTrue b s P I c s1 t)
+    thus ?case using big_step_tr.WhileTrue by auto
+next
+  case (Wait b s P)
+    thus ?case by (simp add: big_step_tr.Wait) 
+qed*)
 
 end
